Formula.v
@@ -3,23 +3,15 @@ Require Import Base Signature Term.
 Section formula.
   Context {Σ : signature}.
 
-  Inductive formula : Type :=
-  | FPred : forall R : PredS Σ, vec (term Σ) (pred_ar R) -> formula
-  | FIndPred : forall R : IndPredS Σ, vec (term Σ) (indpred_ar R) -> formula
-  | FImp : formula -> formula -> formula
-  | FNeg : formula -> formula
-  | FAll : formula -> formula.
-
-  Inductive FV : formula -> E.Ensemble var :=
-  | FV_Pred : forall R args v,
-      V.Forall (fun t => ~ Var t v) args -> FV (FPred R args) v
-  | FV_IndPred : forall R args v,
-      V.Forall (fun t => ~ Var t v) args -> FV (FIndPred R args) v
-  | FV_Imp_l : forall F G v, FV F v -> FV (FImp F G) v
-  | FV_Imp_r : forall F G v, FV G v -> FV (FImp F G) v
-  | FV_Neg : forall F v, FV F v -> FV (FNeg F) v
-  | FV_All : forall F v, FV F v -> FV (FAll F) (S v).
-    
+  Import VarNotations.
+  
+  Inductive formula (X : Vars) : Type :=
+  | FPred : forall R : PredS Σ, vec (term Σ X) (pred_ar R) -> formula X
+  | FIndPred : forall R : IndPredS Σ, vec (term Σ X) (indpred_ar R) -> formula X
+  | FImp : formula X -> formula X -> formula X
+  | FNeg : formula X -> formula X
+  | FAll : formula X⁺ -> formula X.
+   
 End formula.
 
 Arguments formula : clear implicits.
