Structure.v
@@ -1,4 +1,5 @@
 Require Import Base Signature Term.
+Require Import ClassicalDescription.
 
 Section structure.
   Context {Σ : signature}.
@@ -18,61 +19,38 @@ Arguments interpIP {Σ M} _ _ : rename.
 Notation "| M |" := (domain M) (no associativity, at level 150).
 
 Section environment.
-  Context {Σ : signature} {M : structure Σ}.
+  Context {Σ : signature} {X : Vars} {M : structure Σ}.
 
-  Definition env := var -> |M|.
+  Definition env := X -> |M|.
 
-  Definition env_subst (ρ : env) (x : var) (d : |M|) : var -> |M| :=
-    fun (y : var) => if y =? x then d else ρ y.
-
-  Fixpoint eval (ρ : env) (t : term Σ) : |M| :=
+  Import VarNotations.
+  
+  Definition env_subst (ρ : env) (x : X) (d : |M|) : X -> |M| :=
+    fun (y : X) => if y == x then d else ρ y.
+  
+  
+  Fixpoint eval (ρ : env) (t : term Σ X) : |M| :=
     match t with
     | TVar x => ρ x
     | TFunc f args => interpF f (V.map (eval ρ) args)
     end.
 
-  Definition eval_vec (ρ : env) {n} (v : vec (term Σ) n) : vec (|M|) n :=
+  Definition eval_vec (ρ : env) {n} (v : vec (term Σ X) n) : vec (|M|) n :=
     V.map (eval ρ) v.
 
-  Fixpoint eval_subst (ρ : env) (t : term Σ) (x : var) (d : |M|) : |M| :=
+  Fixpoint eval_subst (ρ : env) (t : term Σ X) (x : X) (d : |M|) : |M| :=
     match t with
     | TVar y => env_subst ρ x d y
     | TFunc f args => interpF f (V.map (fun st => eval_subst ρ st x d) args)
     end.
 End environment.
 
-Arguments env {Σ} M.
+Arguments env {Σ} X M.
 
 Section lemma_2_1_5.
-  Context {Σ : signature} {M : structure Σ}.
-  Variable ρ : env M.
-  Variable t : term Σ.
-  Variable x : var.
+  Context {Σ : signature} (X : Vars) {M : structure Σ}.
+  Variable ρ : env X M.
+  Variable t : term Σ X.
+  Variable x : X.
 
-  Lemma eval_subst_sanity1 : forall (d : |M|),
-      ~ Var t x -> eval_subst ρ t x d = eval ρ t.
-  Proof.
-    induction t as [v | f args IH];
-      intros d x_not_in_t.
-    - simpl; unfold env_subst; destruct (v =? x) eqn:eq_vx.
-      + exfalso. apply x_not_in_t. rewrite Nat.eqb_eq in eq_vx; subst.
-        constructor.
-      + reflexivity.
-    - simpl. f_equal. apply V.map_ext_in.
-      intros st Hin. apply IH.
-      + assumption.
-      + intros x_in_var_st. apply x_not_in_t.
-        constructor. apply Exists_exists; exists st; intuition.
-  Qed.
-
-  Lemma eval_subst_sanity2 : forall (u : term Σ),
-      eval_subst ρ t x (eval ρ u) = eval ρ (term_var_subst t x u).
-  Proof.
-    intros u. induction t as [v | f args IH].
-    - cbn. unfold env_subst. destruct (v =? x) eqn:E;
-        reflexivity.
-    - simpl. f_equal. rewrite V.map_map.
-      apply V.map_ext_in. intros st Hst.
-      apply IH. assumption.
-  Qed.
 End lemma_2_1_5.
